coq/Alt_sem.v
@@ -5,7 +5,7 @@
     find this definition more intuitive. *)
 
 Require Import FunInd Program Arith Lia.
-Require Import Monad Proc Alg Sem Sem_tactics.
+Require Import Preamble Monad Proc Alg Sem.
 Import List.ListNotations.
 Open Scope list_scope.
 
