coq/CSem.v
@@ -1,7 +1,7 @@
 (** * Concrete Execution Semantics *)
 
 Require Import FunInd ListSet Arith Program Lia.
-Require Import Monad Proc Alg Sem Sem_tactics.
+Require Import Preamble Monad Proc Alg Sem.
 Import List.ListNotations.
 Open Scope list_scope.
 
